hmac key sizes and other details

src/tls/HKDF.fst
@@ -31,10 +31,10 @@ HKDF-Extract(salt, IKM) -> PRK
 *)
 
 inline_for_extraction
-val extract: 
-  #ha: EverCrypt.HMAC.ha -> 
-  salt: hkey ha -> 
-  ikm: macable ha -> 
+val extract:
+  #ha: EverCrypt.HMAC.ha ->
+  salt: hkey ha ->
+  ikm: macable ha ->
   ST (hkey ha)
   (requires (fun h0 -> True))
   (ensures (fun h0 t h1 -> FStar.HyperStack.modifies Set.empty h0 h1))
@@ -70,10 +70,10 @@ HKDF-Expand(PRK, info, L) -> OKM
 *)
 
 
-val expand: 
-  #ha:Hashing.alg -> 
+val expand:
+  #ha:Hashing.alg ->
   prk: hkey ha ->
-  info: bytes -> 
+  info: bytes ->
   len: UInt32.t {v len <= op_Multiply 255 (tagLength ha)} ->
   Stack (lbytes32 len)
   (requires (fun h0 -> True))
@@ -81,23 +81,23 @@ val expand:
 
 #reset-options "--admit_smt_queries true"
 let expand #ha prk info len =
-  let h00 = HyperStack.ST.get() in 
-  push_frame(); 
+  let h00 = HyperStack.ST.get() in
+  push_frame();
   let tlen = EverCrypt.Hash.tagLen ha in
-  let prk_p = LowStar.Buffer.alloca 0uy tlen in 
+  let prk_p = LowStar.Buffer.alloca 0uy tlen in
   store_bytes prk prk_p;
   assert_norm(EverCrypt.HMAC.keysized ha (EverCrypt.Hash.tagLength ha));
 
   let tag_p = LowStar.Buffer.alloca 0uy len in
-  let infolen = Bytes.len info in 
+  let infolen = Bytes.len info in
 
   if infolen = 0ul then (
-    let info_p = LowStar.Buffer.null in 
+    let info_p = LowStar.Buffer.null in
     EverCrypt.HKDF.hkdf_expand ha tag_p prk_p tlen info_p infolen len
   )
   else (
-    push_frame ();
-    let info_p = LowStar.Buffer.alloca 0uy infolen in 
+    push_frame();
+    let info_p = LowStar.Buffer.alloca 0uy infolen in
     store_bytes info info_p;
     EverCrypt.HKDF.hkdf_expand ha tag_p prk_p tlen info_p infolen len;
     pop_frame ()
@@ -105,10 +105,10 @@ let expand #ha prk info len =
 
   // FIXME(adl) a functional spec would have helped here
   assume False;//18-09-01 not sure what's broken
-    
+
   let tag = of_buffer len tag_p in
   pop_frame();
-  let h11 = HyperStack.ST.get() in 
+  let h11 = HyperStack.ST.get() in
   //18-09-01 todo, as in Hashing.compute
   //assume(HyperStack.modifies Set.empty h00 h11);
   tag
@@ -124,15 +124,15 @@ let expand #ha prk info len =
 /// *last* byte of the concatenated input of HMAC, separating the
 /// domain of the PRF into first blocks and others). On the other
 /// hand, the truncation length is not explicitly encoded here.
-/// 
-private val expand_int: 
+///
+private val expand_int:
   #ha: Hashing.alg -> prk: hkey ha ->
   info: bytes ->
   len: UInt32.t {UInt32.v len <= op_Multiply 255 (tagLength ha)} ->
   count: UInt8.t ->
 //curr: UInt32.t {curr = Int.Cast.uint8_to_uint32 count *^ tagLen ha} ->
   curr: UInt32.t {v curr = op_Multiply (UInt8.v count) (tagLength ha)} ->
-  previous: lbytes32 (if count = 0uy then 0ul else tagLen ha) -> 
+  previous: lbytes32 (if count = 0uy then 0ul else tagLen ha) ->
   ST (b: bytes{
     v len - v curr <= length b /\
     length b <= op_Multiply (UInt8.v count) (blockLength ha)
@@ -142,11 +142,11 @@ private val expand_int:
 
 #set-options "--z3rlimit 10 --admit_smt_queries true"
 let rec expand_int #ha prk info len count curr previous =
-  if curr < len && FStar.UInt8.(count <^ 255uy) then (
+  if curr <^ len && FStar.UInt8.(count <^ 255uy) then (
     assert(FStar.UInt8.(count <^ 255uy));
     assert(UInt8.v count < 255);
     let count = FStar.UInt8.(count +^ 1uy) in
-    let curr = curr + tagLen ha in
+    let curr = curr +^ tagLen ha in
     lemma_repr_bytes_values (UInt8.v count);
     assume (UInt.fits (length previous + length info + 1) 32);
     let block = HMAC.hmac ha prk (previous @| info @| bytes_of_int8 count) in
@@ -157,23 +157,23 @@ let rec expand_int #ha prk info len count curr previous =
 #reset-options
 
 
-// let c32 = FStar.Int.Cast.uint8_to_uint32 count in 
+// let c32 = FStar.Int.Cast.uint8_to_uint32 count in
 //assert (c32 <^ 256ul)
 
-/// Final truncation, possibly chopping of the end of the last block.  
-val expand: 
+/// Final truncation, possibly chopping of the end of the last block.
+val expand2:
   #ha:Hashing.alg -> prk: hkey ha ->
-  info: bytes -> 
+  info: bytes ->
   len: UInt32.t {v len <= op_Multiply 255 (tagLength ha)} ->
   ST (lbytes32 len)
   (requires (fun h0 -> True))
   (ensures (fun h0 t h1 -> FStar.HyperStack.modifies Set.empty h0 h1))
 
 #reset-options "--admit_smt_queries true"
-let expand #ha prk info len =
+let expand2 #ha prk info len =
   lemma_repr_bytes_values (v len);
   let rawbytes = expand_int prk info len 0uy 0ul empty_bytes in
-  fst (split rawbytes len) 
+  fst (split rawbytes len)
 #reset-options
 *)
 
@@ -197,7 +197,7 @@ HKDF-Expand-Label(Secret, Label, Messages, Length) =
 *)
 
 let tls13_prefix : lbytes 6 =
-  let s = bytes_of_string "tls13 " in 
+  let s = bytes_of_string "tls13 " in
   assume(length s = 6); s
 
 let quic_prefix : lbytes 5 =
@@ -206,15 +206,15 @@ let quic_prefix : lbytes 5 =
 
 inline_for_extraction
 val format:
-  ha: Hashing.alg -> 
-  label: string{length (bytes_of_string label) < 256 - 6} -> 
-  hv: bytes{length hv < 256} -> 
+  ha: Hashing.alg ->
+  label: string{length (bytes_of_string label) < 256 - 6} ->
+  hv: bytes{length hv < 256} ->
   len: UInt32.t {v len <= op_Multiply 255 (tagLength ha)} ->
-  is_quic: bool -> 
+  is_quic: bool ->
   Tot bytes
 
 inline_for_extraction
-let format ha label hv len is_quic = 
+let format ha label hv len is_quic =
   let prefix = if is_quic then quic_prefix else tls13_prefix in
   let label_bytes = prefix @| bytes_of_string label in
   lemma_repr_bytes_values (v len);
@@ -222,13 +222,13 @@ let format ha label hv len is_quic =
   lemma_repr_bytes_values (length hv);
   bytes_of_int 2 (v len) @|
   Parse.vlbytes 1 label_bytes @|
-  Parse.vlbytes 1 hv 
+  Parse.vlbytes 1 hv
 
 /// since derivations depend on the concrete info,
-/// we will need to prove format injective. 
+/// we will need to prove format injective.
 
-val expand_label: 
-  #ha: HMAC.ha -> 
+val expand_label:
+  #ha: HMAC.ha ->
   prk: hkey ha ->
   label: string{length (bytes_of_string label) < 256 - 6} -> // -9?
   hv: bytes{length hv < 256} ->
@@ -239,7 +239,7 @@ val expand_label:
   (ensures (fun h0 t h1 -> modifies_none h0 h1))
 
 let expand_label #ha prk label hv len is_quic =
-  expand prk (format ha label hv len is_quic) len 
+  expand prk (format ha label hv len is_quic) len
 
 (*-------------------------------------------------------------------*)
 (*
@@ -260,7 +260,7 @@ val expand_secret:
 
 let expand_secret #ha prk label hv =
   expand_label prk label hv (Hashing.Spec.tagLen ha) false
-  
+
 (*-------------------------------------------------------------------*)
 (*
   Derive-Secret(Secret, Label, Messages) =
@@ -273,7 +273,7 @@ val derive_secret:
   secret: hkey ha ->
   label: string{length (bytes_of_string label) < 256-6} ->
   hs_hash: bytes{length hs_hash < 256} ->
-  is_quic: bool -> 
+  is_quic: bool ->
   ST (lbytes32 (Hashing.Spec.tagLen ha))
   (requires fun h -> True)
   (ensures fun h0 _ h1 -> modifies_none h0 h1)
