src/tls/HMAC.fst
@@ -4,56 +4,63 @@ open Hashing.Spec // for the algorithm names, instead of CoreCrypt
 open Mem
 
 open FStar.HyperStack.ST
-module B = FStar.Bytes
-module LB = LowStar.Buffer
 
-let ha = EverCrypt.HMAC.ha 
+let ha = EverCrypt.HMAC.ha
 
 (* Parametric keyed HMAC; could be coded up from two HASH calls. *)
 
 val hmac:
-  a:ha -> 
-  k:hkey a -> 
-  m: macable a -> 
+  a:ha ->
+  k:hkey a ->
+  m: macable a ->
+//18-09-12 failing on equal_domains with Stack instead of ST, not sure why.
   ST (tag a)
   (requires fun h0 -> True)
-  (ensures fun h0 t h1 -> 
-    modifies_none h0 h1 /\ // FIXME this is now wrong
+  (ensures fun h0 t h1 ->
+    modifies_none h0 h1 /\ // FIXME(adl) this is now wrong
     t = Hashing.Spec.hmac a k m)
 
 #set-options "--z3rlimit 20"
-let hmac a k m = 
-  let h00 = get() in 
-  push_frame(); 
+let hmac a k m =
+  let h00 = get() in
+  push_frame();
   let lt = EverCrypt.Hash.tagLen a in
-  let lk = B.len k in
-  let bk = LB.alloca 0uy lk in 
-  B.store_bytes k bk;
-  let bt = LB.alloca 0uy lt in
-  let lm = B.len m in 
+  let lk = Bytes.len k in
+  let bk = LowStar.Buffer.alloca 0uy lk in
+  Bytes.store_bytes k bk;
+  let bt = LowStar.Buffer.alloca 0uy lt in
+  let lm = Bytes.len m in
 
   if lm = 0ul then (
-    B.empty_unique m;
-    EverCrypt.HMAC.compute a bt bk lk LB.null lm;
-    let h1 = get() in
-    assume(LB.as_seq h1 bt == B.reveal (Hashing.Spec.hmac a k m))
-  ) else (
+    let bm = LowStar.Buffer.null in
+    let h0 = get() in
+    Seq.lemma_eq_intro (Bytes.reveal m) (LowStar.Buffer.as_seq h0 bm);
+    EverCrypt.HMAC.compute a bt bk lk bm lm
+  )
+  else (
+    let h0 = get() in
     push_frame();
-    let bm = LB.alloca 0uy lm in 
-    B.store_bytes m bm;
+    let bm = LowStar.Buffer.alloca 0uy lm in
+    Bytes.store_bytes m bm;
     EverCrypt.HMAC.compute a bt bk lk bm lm;
-    pop_frame()
-  );
+    pop_frame();
+    let h1 = get() in
+    assert(LowStar.Modifies.(modifies (loc_buffer bt) h0 h1))
+    //assume(equal_domains h0 h1)
+    );
 
-  let h2 = get() in
-  assert(LB.as_seq h2 bt == B.reveal (Hashing.Spec.hmac a k m));
-  let t = B.of_buffer lt bt in
+  let t = Bytes.of_buffer lt bt in
+  assert(Bytes.reveal t == EverCrypt.HMAC.hmac a (Bytes.reveal k) (Bytes.reveal m));
+  assert(t = Hashing.Spec.hmac a k m);
   pop_frame();
-  let h11 = get() in
-  assume(modifies_none h00 h11); // FIXME
+  let h11 = HyperStack.ST.get() in
+  //18-09-01 todo, as in Hashing.compute
+  assert(LowStar.Modifies.(modifies loc_none h00 h11));
+  assume(modifies_none h00 h11); //18-09-12 missing compatibility lemma?
   t
 
-//18-09-02 TODO lower code to avoid bytes-allocating the tag. 
+
+//18-09-02 TODO lower code to avoid bytes-allocating the tag.
 
 val hmacVerify: a:ha -> k:hkey a -> m:macable a -> t: tag a -> ST (b:bool {b <==> (t == Hashing.Spec.hmac a k m)})
   (requires (fun h0 -> True))
@@ -62,6 +69,7 @@ val hmacVerify: a:ha -> k:hkey a -> m:macable a -> t: tag a -> ST (b:bool {b <==
 let hmacVerify a k p t =
   let result = hmac a k p in
   result = t
+
 
 /// Historical constructions from SSL, still used in TLS 1.0, actually
 /// just HMAC. Disable in this version of the code.
@@ -80,14 +88,14 @@ let sslKeyedHashPads = function
     | Hash MD5 -> (ssl_pad1_md5, ssl_pad2_md5)
     | Hash SHA1 -> (ssl_pad1_sha1, ssl_pad2_sha1)
 
-private val sslKeyedHash: 
-  a:alg {a=MD5 \/ a=SHA1} -> 
+private val sslKeyedHash:
+  a:alg {a=MD5 \/ a=SHA1} ->
   k:hkey a -> text a -> ST (tag a)
   (requires fun h0 -> True)
   (ensures fun h0 t h1 -> modifies_none h0 h1)
 let sslKeyedHash a k p =
-    let (inner, outer) = 
-      match a with 
+    let (inner, outer) =
+      match a with
       | MD5 -> ssl_pad1_md5, ssl_pad2_md5
       | SHA1 -> ssl_pad1_sha1, ssl_pad2_sha1 in
 
@@ -96,9 +104,9 @@ let sslKeyedHash a k p =
     let h = Hashing.compute a (k @| inner @| p) in
     Hashing.compute a (k @| outer @| h)
 
-private val sslKeyedHashVerify: 
-  a:alg {a=MD5 \/ a=SHA1} -> 
-  k:hkey a -> text a -> t:tag a -> ST bool 
+private val sslKeyedHashVerify:
+  a:alg {a=MD5 \/ a=SHA1} ->
+  k:hkey a -> text a -> t:tag a -> ST bool
   (requires fun h0 -> True)
   (ensures fun h0 t h1 -> modifies Set.empty h0 h1)
 let sslKeyedHashVerify a k p t =
@@ -110,24 +118,23 @@ let sslKeyedHashVerify a k p t =
 
 /// Agile bytes-friendly MAC function
 
-type macable = b:B.bytes {B.length b + 128 < pow2 32} // [==> pre of hmac for all algorithms]
+type macable = b:Bytes.bytes {Bytes.length b + 128 < pow2 32} // [==> pre of hmac for all algorithms]
 
-val tls_mac: a: 
-  tls_macAlg -> 
-  k: hkey a  -> 
-  msg:macable -> 
+val tls_mac: a:
+  tls_macAlg ->
+  k: hkey a  ->
+  msg:macable ->
   ST (tag a)
   (requires fun h0 -> True)
   (ensures fun h0 t h1 -> FStar.HyperStack.modifies Set.empty h0 h1)
 let tls_mac a k msg  = hmac a k msg
 
-val tls_macVerify: 
-  a:tls_macAlg -> 
-  k: hkey a  -> 
-  msg:macable -> 
-  tag a -> 
+val tls_macVerify:
+  a:tls_macAlg ->
+  k: hkey a  ->
+  msg:macable ->
+  tag a ->
   ST bool
   (requires fun h0 -> True)
   (ensures (fun h0 t h1 -> FStar.HyperStack.modifies Set.empty h0 h1))
 let tls_macVerify a k d t = hmacVerify a k d t
-
